Add `rankMatroid_rel_rank_eq_matroid_rel_Rank` WIP

Matroid/Constructions/RankAxioms.lean
@@ -9,73 +9,79 @@ structure RankMatroid (α : Type*) where
   /-- The (relative) rank function -/
   (relRank : Set α → Set α → ℕ∞)
 
-  (relRank_le_encard_diff {A B : Set α} : A ⊆ E → B ⊆ A → relRank A B ≤ (A \ B).encard)
-  (relRank_union_le_relRank_inter {A B : Set α} : A ⊆ E → B ⊆ E → relRank (A ∪ B) B ≤ relRank A (A ∩ B))
-  (relRank_add_cancel {A B C : Set α} : A ⊆ E → B ⊆ A → C ⊆ B → (relRank A C) = (relRank A B) + (relRank B C))
-  (relRank_sUnion_eq_zero {S : Set (Set α)} {B : Set α} :
+  (rel_rank_le_encard_diff {A B : Set α} : A ⊆ E → B ⊆ A → relRank A B ≤ (A \ B).encard)
+  (rel_rank_union_le_relRank_inter {A B : Set α} : A ⊆ E → B ⊆ E → relRank (A ∪ B) B ≤ relRank A (A ∩ B))
+  (rel_rank_add_cancel {A B C : Set α} : A ⊆ E → B ⊆ A → C ⊆ B → (relRank A C) = (relRank A B) + (relRank B C))
+  (rel_rank_sUnion_eq_zero {S : Set (Set α)} {B : Set α} :
       (∀ A ∈ S, B ⊆ A ∧ A ⊆ E ∧ relRank A B = 0) → relRank (⋃₀ S) B = 0)
 
-  (RIndep : Set α → Prop)
-  (rindep_maximal : ∀ X ⊆ E, Matroid.ExistsMaximalSubsetProperty RIndep X)
-  (rindep_iff' : ∀ I, RIndep I ↔ I ⊆ E ∧ ∀ x ∈ I, relRank I (I \ {x}) > 0 )
+  (Indep : Set α → Prop)
+  (indep_maximal : ∀ X ⊆ E, Matroid.ExistsMaximalSubsetProperty Indep X)
+  (indep_iff' : ∀ I, Indep I ↔ I ⊆ E ∧ ∀ x ∈ I, relRank I (I \ {x}) > 0 )
 
 namespace RankMatroid
 
 variable {α : Type*} {A B I J X : Set α} {M : RankMatroid α} {x : α}
 
+def indepSubsets (M : RankMatroid α) (A : Set α) : Set (Set α) :=
+  {I | M.Indep I ∧ I ⊆ A}
+
+def Basis' (M : RankMatroid α) (I A : Set α) : Prop :=
+  I ∈ maximals (· ⊆ ·) (M.indepSubsets A)
+
 theorem r_nonneg : M.relRank A B ≥ 0 := by
   exact zero_le (M.relRank A B)
 
 theorem relRank_self_eq_zero (h : A ⊆ M.E) : M.relRank A A = 0 := by
-  have := M.relRank_le_encard_diff h (subset_refl A)
+  have := M.rel_rank_le_encard_diff h (subset_refl A)
   rw [Set.diff_eq_empty.mpr fun ⦃a⦄ a ↦ a, Set.encard_empty] at this
   exact nonpos_iff_eq_zero.mp this
 
-theorem RIndep.subset_ground (h : M.RIndep I) : I ⊆ M.E := by
-  rw [rindep_iff'] at h
+theorem Indep.subset_ground (h : M.Indep I) : I ⊆ M.E := by
+  rw [indep_iff'] at h
   exact h.left
 
-theorem RIndep.indep (h : M.RIndep I) :  ∀ x ∈ I, M.relRank I (I \ {x}) > 0  := by
-  rw [rindep_iff'] at h
+theorem Indep.indep (h : M.Indep I) :  ∀ x ∈ I, M.relRank I (I \ {x}) > 0  := by
+  rw [indep_iff'] at h
   exact h.right
 
-theorem indep_subset (hJ : M.RIndep J) (rIJ : I ⊆ J) : M.RIndep I := by
-    rw [M.rindep_iff']
-    refine ⟨rIJ.trans hJ.subset_ground, λ x hx ↦ ?_⟩
-    have hJ_indep := hJ.subset_ground
-    have hJ := hJ.indep x (Set.mem_of_mem_of_subset hx rIJ)
-    set A := I
-    set B := J \ {x}
-    have hAUB : J = A ∪ B := by
-      refine (Set.union_diff_cancel' ?h₁ rIJ).symm
-      exact Set.singleton_subset_iff.mpr hx
-    have hAIB : A \ {x} = A ∩ B := by
-      ext y;
-      refine ⟨λ hY ↦ ?_, λ hY ↦ ?_⟩
-      · refine ⟨Set.mem_of_mem_diff hY, Set.mem_diff_singleton.mpr ?_⟩
-        refine ⟨rIJ (Set.mem_of_mem_diff hY), ?_⟩
-        have h := Set.not_mem_of_mem_diff hY
-        exact h
-      have hyB : y ∈ J \ {x} := Set.mem_of_mem_inter_right hY
-      have hynex : y ≠ x := by have := Set.not_mem_of_mem_diff hyB; exact this
-      exact ⟨Set.mem_of_mem_inter_left hY, hynex⟩
-    rw [hAUB] at hJ
-    rw [hAIB]
-    have hA : A ⊆ M.E := (rIJ.trans hJ_indep)
-    have hB : B ⊆ M.E := ((Set.diff_subset J {x}).trans hJ_indep)
-    exact hJ.trans_le (M.relRank_union_le_relRank_inter hA hB)
+theorem indep_subset (hJ : M.Indep J) (rIJ : I ⊆ J) : M.Indep I := by
+  rw [M.indep_iff']
+  refine ⟨rIJ.trans hJ.subset_ground, fun x hx ↦ ?_⟩
+  have hJ_indep := hJ.subset_ground
+  have hJ := hJ.indep x (Set.mem_of_mem_of_subset hx rIJ)
+  set A := I
+  set B := J \ {x}
+  have hAUB : J = A ∪ B := by
+    refine (Set.union_diff_cancel' ?h₁ rIJ).symm
+    exact Set.singleton_subset_iff.mpr hx
+  have hAIB : A \ {x} = A ∩ B := by
+    ext y;
+    refine ⟨fun hY ↦ ?_, fun hY ↦ ?_⟩
+    · refine ⟨Set.mem_of_mem_diff hY, Set.mem_diff_singleton.mpr ?_⟩
+      refine ⟨rIJ (Set.mem_of_mem_diff hY), ?_⟩
+      have h := Set.not_mem_of_mem_diff hY
+      exact h
+    have hyB : y ∈ J \ {x} := Set.mem_of_mem_inter_right hY
+    have hynex : y ≠ x := by have := Set.not_mem_of_mem_diff hyB; exact this
+    exact ⟨Set.mem_of_mem_inter_left hY, hynex⟩
+  rw [hAUB] at hJ
+  rw [hAIB]
+  have hA : A ⊆ M.E := (rIJ.trans hJ_indep)
+  have hB : B ⊆ M.E := ((Set.diff_subset J {x}).trans hJ_indep)
+  exact hJ.trans_le (M.rel_rank_union_le_relRank_inter hA hB)
 
 theorem r_le_r_subset_right (hX : X ⊆ M.E) (hAX : A ⊆ X) (hBA : B ⊆ A) : M.relRank X A ≤ M.relRank X B := by
-  rw [M.relRank_add_cancel hX hAX hBA]; simp
+  rw [M.rel_rank_add_cancel hX hAX hBA]; simp only [self_le_add_right]
 
-theorem insert_indep_iff_r_insert_pos (hI_indep : M.RIndep I) (hx : x ∈ M.E \ I)
-    : M.RIndep (Set.insert x I) ↔ M.relRank (Set.insert x I) I > 0 := by
-  refine ⟨λ hIx_indep ↦ ?_, λ hr ↦ ?_⟩
+theorem insert_indep_iff_r_insert_pos (hI_indep : M.Indep I) (hx : x ∈ M.E \ I)
+    : M.Indep (Set.insert x I) ↔ M.relRank (Set.insert x I) I > 0 := by
+  refine ⟨fun hIx_indep ↦ ?_, fun hr ↦ ?_⟩
   · have h := hIx_indep.indep x (Set.mem_insert x I)
     have : Set.insert x I \ {x} = I :=
       Set.insert_diff_self_of_not_mem (Set.not_mem_of_mem_diff hx)
     rwa [this] at h
-  refine (M.rindep_iff' (Set.insert x I)).mpr ?_
+  refine (M.indep_iff' (Set.insert x I)).mpr ?_
   refine ⟨Set.insert_subset (Set.mem_of_mem_diff hx) hI_indep.subset_ground, ?_⟩
   contrapose! hr
   rcases hr with ⟨y, hy, hr⟩
@@ -95,18 +101,18 @@ theorem insert_indep_iff_r_insert_pos (hI_indep : M.RIndep I) (hx : x ∈ M.E \ 
       rw [Set.insert_diff_singleton]
       exact (Set.subset_insert x I).trans (Set.subset_insert y (Set.insert x I))
     have hrBC : M.relRank B C ≤ 1 := by
-      have h := M.relRank_le_encard_diff (h₂.trans h₁) h₃
+      have h := M.rel_rank_le_encard_diff (h₂.trans h₁) h₃
       rw [Set.diff_diff_right] at h
       have h := h.trans (Set.encard_union_le (B \ I) (B ∩ {y}))
       rw [Set.encard_eq_zero.mpr Set.diff_inter_self] at h
       simp only [add_zero] at h
-      have : B \ I ⊆ {x} := by refine Set.diff_subset_iff.mpr ?_; simp; exact h₂
+      have : B \ I ⊆ {x} := by refine Set.diff_subset_iff.mpr ?_; simp only [Set.union_singleton]; exact h₂
       rcases Set.subset_singleton_iff_eq.mp this with h' | h'
       · rw [h'] at h; rw [Set.encard_empty] at h; exact h.trans zero_le_one
       rw [h'] at h; rwa [Set.encard_singleton] at h;
     have h : M.relRank A B + M.relRank B C <= 1 := by
       exact add_le_add hr hrBC
-    have := M.relRank_add_cancel h₁ h₂ h₃
+    have := M.rel_rank_add_cancel h₁ h₂ h₃
     rwa [<-this] at h
   set A := (Set.insert x I)
   set B := (I)
@@ -115,7 +121,7 @@ theorem insert_indep_iff_r_insert_pos (hI_indep : M.RIndep I) (hx : x ∈ M.E \ 
     have h₁ : A ⊆ M.E := Set.insert_subset (Set.mem_of_mem_diff hx) hI_indep.subset_ground
     have h₂ : B ⊆ A := Set.subset_insert x I
     have h₃ : C ⊆ B := Set.diff_subset I {y}
-    exact M.relRank_add_cancel h₁ h₂ h₃
+    exact M.rel_rank_add_cancel h₁ h₂ h₃
   have h'' : M.relRank B C ≥ 1 := by
     rcases Set.mem_insert_iff.mp hy with rfl | hy
     · contradiction
@@ -130,9 +136,9 @@ theorem insert_indep_iff_r_insert_pos (hI_indep : M.RIndep I) (hx : x ∈ M.E \ 
   refine (ENat.add_one_le_iff ?refine_2.intro.intro.hm).mp this
   exact ENat.coe_toNat_eq_self.mp rfl
 
-theorem indep_subset_maximal_iff_relrank_zero (hX : X ⊆ M.E) (hI : I ⊆ X) (hI_indep : M.RIndep I) :
-    (I ∈ (maximals (· ⊆ ·) {S | M.RIndep S ∧ S ⊆ X}) ↔ M.relRank X I = 0) := by
-  refine ⟨λ hI_max ↦ ?_, λ hr ↦ ?_⟩
+theorem indep_subset_maximal_iff_relrank_zero (hX : X ⊆ M.E) (hI : I ⊆ X) (hI_indep : M.Indep I) :
+    (I ∈ (maximals (· ⊆ ·) {S | M.Indep S ∧ S ⊆ X}) ↔ M.relRank X I = 0) := by
+  refine ⟨fun hI_max ↦ ?_, fun hr ↦ ?_⟩
   · by_cases hXI : X = I
     · rw [hXI]; exact relRank_self_eq_zero hI_indep.subset_ground
     set S := {(insert x I) | x ∈ X \ I}
@@ -142,14 +148,14 @@ theorem indep_subset_maximal_iff_relrank_zero (hX : X ⊆ M.E) (hI : I ⊆ X) (h
       refine ⟨Set.subset_insert x I, Set.insert_subset (hX hxX) hI_indep.subset_ground, ?_⟩
       contrapose! hI_max
       have hI_max : M.relRank (insert x I) I > 0 := by exact pos_iff_ne_zero.mpr hI_max
-      suffices h : M.RIndep (insert x I) by
-        have : (insert x I) ∈ {S | M.RIndep S ∧ S ⊆ X} := ⟨h, Set.insert_subset hxX hI⟩
+      suffices h : M.Indep (insert x I) by
+        have : (insert x I) ∈ {S | M.Indep S ∧ S ⊆ X} := ⟨h, Set.insert_subset hxX hI⟩
         apply mem_maximals_iff.not.mpr
         push_neg; intro; use (insert x I)
         exact ⟨this, Set.subset_insert x I, by exact Set.ne_insert_of_not_mem I hxI⟩
       have hxEI : x ∈ M.E \ I := by exact (Set.mem_diff x).mpr ⟨hX hxX, hxI⟩
       exact (insert_indep_iff_r_insert_pos hI_indep hxEI).mpr hI_max
-    have := M.relRank_sUnion_eq_zero h
+    have := M.rel_rank_sUnion_eq_zero h
     have hXU : X = S.sUnion := by
       apply Set.eq_of_subset_of_subset
       · intro x hx; simp only [Set.mem_sUnion]
@@ -170,26 +176,27 @@ theorem indep_subset_maximal_iff_relrank_zero (hX : X ⊆ M.E) (hI : I ⊆ X) (h
       exact Set.insert_subset ((Set.mem_diff x).mpr hx_mem).left hI
     rwa [<-hXU] at this
   contrapose! hr
-  unfold maximals at hr; simp at hr
+  unfold maximals at hr;
+  simp only [Set.mem_setOf_eq, and_imp, not_and, not_forall, Classical.not_imp, exists_prop, exists_and_left] at hr
   obtain ⟨I', hI'_indep, hI', hI'_ssubset⟩ := hr hI_indep hI
   rw [<-Set.ssubset_def] at hI'_ssubset
   obtain ⟨x, hxI', hxI⟩ := Set.exists_of_ssubset hI'_ssubset
-  have : M.RIndep (Set.insert x I) := by
+  have : M.Indep (Set.insert x I) := by
     exact indep_subset hI'_indep (Set.insert_subset hxI' hI'_ssubset.subset)
   rw [insert_indep_iff_r_insert_pos hI_indep ((Set.mem_diff x).mpr ⟨(hI'.trans hX) hxI', hxI⟩)] at this
   have : M.relRank X I > 0 := by
-    rw [M.relRank_add_cancel hX (Set.insert_subset (hI' hxI') hI) (Set.subset_insert x I)]
+    rw [M.rel_rank_add_cancel hX (Set.insert_subset (hI' hxI') hI) (Set.subset_insert x I)]
     have this' : M.relRank X (Set.insert x I) ≥ 0 := by exact r_nonneg
     exact Right.add_pos_of_nonneg_of_pos this' this
   exact pos_iff_ne_zero.mp this
 
-@[simps] protected def matroid (M : RankMatroid α) : IndepMatroid α where
+@[simps] protected def indepMatroid (M : RankMatroid α) : IndepMatroid α where
   E := M.E
-  Indep := M.RIndep
+  Indep := M.Indep
 
   indep_empty := by
-    rw [M.rindep_iff'];
-    refine ⟨Set.empty_subset M.E, λ x hx ↦ ?_⟩
+    rw [M.indep_iff'];
+    refine ⟨Set.empty_subset M.E, fun x hx ↦ ?_⟩
     contradiction
 
   indep_subset := by
@@ -197,10 +204,10 @@ theorem indep_subset_maximal_iff_relrank_zero (hX : X ⊆ M.E) (hI : I ⊆ X) (h
     exact indep_subset hJ rIJ
 
   indep_aug := by
-    have hiff : {S | M.RIndep S ∧ S ⊆ M.E} = {S | M.RIndep S} := by
+    have hiff : {S | M.Indep S ∧ S ⊆ M.E} = {S | M.Indep S} := by
       ext S; constructor
-      · simp; tauto
-      simp; exact λ h ↦ ⟨h, h.subset_ground⟩
+      · simp only [Set.mem_setOf_eq, and_imp]; tauto
+      simp only [Set.mem_setOf_eq]; exact fun h ↦ ⟨h, h.subset_ground⟩
 
     intro I B hI_indep hI_nmax hB_max
     have hB_indep := (mem_maximals_iff.mp hB_max).left
@@ -221,22 +228,22 @@ theorem indep_subset_maximal_iff_relrank_zero (hX : X ⊆ M.E) (hI : I ⊆ X) (h
       calc
       0 < M.relRank M.E I := by assumption
       _ = M.relRank M.E (I ∪ B) + M.relRank (I ∪ B) I := by
-        exact M.relRank_add_cancel h₃ h₂ h₁
+        exact M.rel_rank_add_cancel h₃ h₂ h₁
       _ ≤ M.relRank M.E B + M.relRank (I ∪ B) I := by
         apply add_le_add_right
         exact r_le_r_subset_right h₃ h₂ (Set.subset_union_right I B)
       _ = M.relRank (I ∪ B) I := by
         rw [hrEB]
-        simp
+        simp only [zero_add]
     have hIUB_subset := (Set.union_subset hI_indep.subset_ground hB_indep.subset_ground)
     have hI_nmax := (not_iff_not.mpr (indep_subset_maximal_iff_relrank_zero hIUB_subset (Set.subset_union_left I B) hI_indep)).mpr (Ne.symm (hrIUB_I.ne))
-    have h_maximals_nonempty := M.rindep_maximal (I ∪ B) hIUB_subset I hI_indep  (Set.subset_union_left I B)
+    have h_maximals_nonempty := M.indep_maximal (I ∪ B) hIUB_subset I hI_indep  (Set.subset_union_left I B)
     rcases h_maximals_nonempty with ⟨I', ⟨hI'_indep, hI'_contains_I, hI'_in_IUB⟩, hI'_max⟩
     by_cases hII' : I = I'
     · rw [<-hII'] at hI'_max hI'_indep
-      simp at hI'_max
+      simp only [Set.mem_setOf_eq, and_imp] at hI'_max
       contrapose! hI_nmax
-      rw [mem_maximals_iff]; simp
+      rw [mem_maximals_iff]; simp only [Set.mem_setOf_eq, Set.subset_union_left, and_true, and_imp]
       refine ⟨by assumption, ?_⟩
       intro y hy_indep hy_in hy_within
       have := hI'_max hy_indep hy_within hy_in hy_within
@@ -252,7 +259,163 @@ theorem indep_subset_maximal_iff_relrank_zero (hX : X ⊆ M.E) (hI : I ⊆ X) (h
     refine ⟨this, ?_⟩
     exact indep_subset hI'_indep (Set.insert_subset hx.left hI'_contains_I)
 
-  indep_maximal := λ X hX ↦ M.rindep_maximal X hX
-  subset_ground := λ I hI ↦ hI.subset_ground
+  indep_maximal := fun X hX ↦ M.indep_maximal X hX
+  subset_ground := fun I hI ↦ hI.subset_ground
+
+@[simps] protected def matroid (M : RankMatroid α) : Matroid α := M.indepMatroid.matroid
+
+end RankMatroid
+
+namespace Matroid
+
+variable {α : Type*} {I : Set α}
+
+def indepSubsets (M : Matroid α) (A : Set α) : Set (Set α) :=
+  {I | M.Indep I ∧ I ⊆ A}
+
+noncomputable def relRank (M : Matroid α) (A B : Set α) : ℕ∞ :=
+  sSup {x | ∃ I J : Set α, J ⊆ I ∧ I ∈ M.indepSubsets A ∧ M.Basis' J B ∧ x = (I \ J).encard}
+
+theorem basis_of_maximal_extension (M : Matroid α) {I X J : Set α} (hX : X ⊆ M.E) (hI : I ⊆ X) (hI_indep : M.Indep I)
+    (h : J ∈ maximals (· ⊆ ·) {I' | M.Indep I' ∧ I ⊆ I' ∧ I' ⊆ X}) : M.Basis' J X := by
+  unfold Basis'; unfold maximals at h ⊢; simp only [Set.mem_setOf_eq, and_imp] at h ⊢
+  obtain ⟨⟨hJ_indep, hIJ, hJX⟩, hJ_max⟩ := h
+  refine ⟨⟨hJ_indep, hJX⟩, ?_⟩
+  intro J' hJ'_indep hJ'X hJJ'
+  exact hJ_max hJ'_indep (hIJ.trans hJJ') hJ'X hJJ'
+
+theorem rel_rank_eq_any_choice (M : Matroid α) {A B : Set α} (hB : B ⊆ A) (hA : A ⊆ M.E) {I J : Set α}
+    (h : J ⊆ I) (hI : M.Basis' I A) (hJ : M.Basis' J B) :
+    M.relRank A B = (I \ J).encard := by
+  unfold Basis' maximals at hJ; simp only [Set.mem_setOf_eq, and_imp] at hJ
+  have ⟨⟨hJ_indep, hJ_subset_B⟩, hJ_max⟩ := hJ
+  apply le_antisymm_iff.mpr; rw [and_comm]
+  constructor
+  · have : (I \ J).encard ∈ {x | ∃ I J : Set α, J ⊆ I ∧ I ∈ M.indepSubsets A ∧ J ∈ maximals (· ⊆ ·) (M.indepSubsets B) ∧ x = (I \ J).encard} := by
+      use I, J; unfold maximals indepSubsets; simp only [Set.mem_setOf_eq, and_imp, and_true];
+      unfold Basis' at hI
+      exact ⟨h, (maximals_subset (fun a b ↦ a ⊆ b) (M.indepSubsets A)) hI, hJ.1, hJ.2⟩
+    exact le_sSup this
+  apply sSup_le; intro r; simp only [Set.mem_setOf_eq, forall_exists_index, and_imp]
+  rintro I' J' h' hI' hJ' rfl
+  sorry
+
+theorem rel_rank_exists (M : Matroid α) {A B : Set α} (hB : B ⊆ A) (hA : A ⊆ M.E) :
+    ∃ I J : Set α, J ⊆ I ∧ M.Basis' I A ∧ M.Basis' J B ∧ M.relRank A B = (I \ J).encard := by
+  obtain ⟨J, hJ⟩ := M.maximality B (hB.trans hA) ∅ M.empty_indep (Set.empty_subset B)
+  unfold maximals at hJ; simp only [Set.empty_subset, true_and, Set.mem_setOf_eq, and_imp] at hJ
+  have ⟨⟨hJ_indep, hJ_subset_B⟩, hJ_max⟩ := hJ
+  obtain ⟨I, hI⟩ := M.maximality A hA J hJ_indep (hJ_subset_B.trans hB)
+  use I; use J
+  unfold Basis'
+  have hIJ : J ⊆ I := hI.1.2.1
+  have hI_basis : M.Basis' I A := by
+    refine M.basis_of_maximal_extension hA (hJ.1.2.trans hB) hJ.1.1 hI
+  have hJ_basis : M.Basis' J B := by
+    refine M.basis_of_maximal_extension (hB.trans hA) (Set.empty_subset B) M.empty_indep ?_
+    unfold maximals; simp only [Set.empty_subset, true_and, Set.mem_setOf_eq, and_imp]
+    assumption
+  exact ⟨hIJ, hI_basis, hJ_basis, M.rel_rank_eq_any_choice hB hA hIJ hI_basis hJ_basis⟩
+
+end Matroid
+
+namespace RankMatroid
+
+variable {α : Type*} {A B I J X : Set α} {M : RankMatroid α} {x : α}
+
+theorem relRank_indeps_eq_encard_diff (M : RankMatroid α) {A B : Set α} (hB : B ⊆ A) (hA : M.Indep A)
+    : M.relRank A B = (A \ B).encard := by
+  set P := fun n ↦ ∀ (A B : Set α), B ⊆ A → M.Indep A → (A \ B).encard = n → M.relRank A B = n
+  have h_induc : ∀ n : ℕ∞, P n := by
+    intro n
+    refine (@ENat.nat_induction P n ?_ ?_ ?_)
+    · intro A B hB hA_indep h
+      have := M.rel_rank_le_encard_diff hA_indep.subset_ground hB
+      rw [h] at this; simp only [nonpos_iff_eq_zero] at this; assumption
+    · intro n hPn A B hB hA_indep h
+      have : (n.succ : ℕ∞) > 0 := by exact NeZero.pos (n.succ : ℕ∞)
+      rw [<-h] at this
+      rcases (Set.encard_pos.mp this) with ⟨x, hx⟩
+      set A' := A \ {x}
+      have hxA : x ∈ A := Set.mem_of_mem_diff hx
+      have hAA' : A' ⊆ A := by exact Set.diff_subset A {x}
+      have hBA' : B ⊆ A' := Set.subset_diff_singleton hB (Set.not_mem_of_mem_diff hx)
+      have hA'_indep : M.Indep A' := M.indep_subset hA_indep hAA'
+      have hA'dB: A' \ B = (A \ B) \ {x} := by exact Set.diff_diff_comm
+      have : (A' \ B).encard = n := by
+        rw [hA'dB]
+        rw [<-Set.encard_diff_singleton_add_one hx] at h
+        simp only [Nat.succ_eq_add_one, Nat.cast_add, Nat.cast_one] at h
+        exact WithTop.add_right_cancel (ENat.coe_toNat_eq_self.mp (refl 1)) h
+      have hrA'B : M.relRank A' B = n := hPn A' B hBA' hA'_indep this
+      have hrAA' : M.relRank A A' = 1 := by
+        have hle : M.relRank A A' <= 1 := by
+          have := M.rel_rank_le_encard_diff hA_indep.subset_ground (Set.diff_subset A {x})
+          rw [Set.diff_diff_cancel_left (Set.singleton_subset_iff.mpr hxA)] at this
+          simp at this; exact this
+        have hgt : M.relRank A A' > 0 := by exact hA_indep.indep x hxA
+        refine le_antisymm_iff.mpr ⟨hle, ENat.one_le_iff_pos.mpr hgt⟩
+      rw [M.rel_rank_add_cancel hA_indep.subset_ground hAA' hBA', hrA'B, hrAA']
+      have h11: (1 : ℕ) = (1 : ℕ∞) := rfl
+      rw [<-h11, <-(ENat.coe_add 1 n), add_comm, Nat.succ_eq_add_one];
+    intro hP A B hB hA_indep h
+    by_contra! h_finite
+    rcases Option.ne_none_iff_exists'.mp h_finite with ⟨c, hc⟩
+    simp at h
+    obtain ⟨D, hD_subset, hD_finite, hD_ncard⟩ := Set.Infinite.exists_subset_ncard_eq h (c+1)
+    have hD_encard : D.encard = c+1 := by
+      have : (c + 1 : ℕ) = (c + 1 : ℕ∞) := rfl
+      rw [<-this];
+      have : (D.ncard : ℕ∞) = (c + 1 : ℕ∞) := by exact congrArg Nat.cast hD_ncard
+      have : D.encard = (D.ncard : ℕ∞) := by exact Eq.symm (Set.Finite.cast_ncard_eq hD_finite)
+      rw [this]
+      assumption
+    clear hD_ncard hD_finite h_finite
+    let B' := B ∪ D
+    have hD_subset_A : D ⊆ A := hD_subset.trans (Set.diff_subset A B)
+    have hD_indep : M.Indep D := by exact M.indep_subset hA_indep hD_subset_A
+    have hB'_subset_A : B' ⊆ A := by exact (Set.union_subset hB hD_subset_A)
+    have hB'_indep : M.Indep B' := by exact M.indep_subset hA_indep hB'_subset_A
+    have hB'B : (B' \ B).encard = c + 1 := by
+      have : B ∩ D ⊆ ∅ := by
+        have : Disjoint B (A \ B) := Set.disjoint_sdiff_right
+        have : Disjoint B D := by exact Set.disjoint_of_subset (fun ⦃a⦄ a ↦ a) hD_subset this
+        exact Set.disjoint_iff.mp this
+      rwa [Set.union_diff_cancel_left this]
+    have hrB'B : M.relRank B' B = c + 1 := hP (c+1) B' B (Set.subset_union_left B D) hB'_indep hB'B
+    have hbad : M.relRank A B ≥ c + 1 := by
+      rw [M.rel_rank_add_cancel hA_indep.subset_ground hB'_subset_A (Set.subset_union_left B D), hrB'B]
+      simp only [ge_iff_le, self_le_add_left]
+    rw [hc] at hbad;
+    have : c ≥ c + 1 := by exact WithTop.some_le_some.mp hbad
+    linarith
+  exact h_induc (A \ B).encard A B hB hA rfl
+
+theorem rankMatroid_rel_rank_eq_matroid_rel_rank (M : RankMatroid α)
+    {A B : Set α} (hB : B ⊆ A) (hA : A ⊆ M.E): M.relRank A B = M.matroid.relRank A B := by
+  obtain ⟨I, J, hJ, hI_basis_A, hJ_basis_B, h⟩ := M.matroid.rel_rank_exists hB hA
+  rw [h]; clear h;
+  unfold Matroid.Basis' maximals at hI_basis_A hJ_basis_B;
+  simp only [matroid_Indep, Set.mem_setOf_eq, and_imp] at hI_basis_A hJ_basis_B
+  obtain ⟨⟨hI_indep, hI_subset⟩, hI_max⟩ := hI_basis_A
+  obtain ⟨⟨hJ_indep, hJ_subset⟩, hJ_max⟩ := hJ_basis_B
+  rw [<-M.relRank_indeps_eq_encard_diff hJ hI_indep]
+  have hAI : M.relRank A I = 0 := by
+    rw [<-indep_subset_maximal_iff_relrank_zero hA hI_subset hI_indep]
+    unfold maximals; simp only [Set.mem_setOf_eq, and_imp]
+    exact ⟨⟨hI_indep, hI_subset⟩, hI_max⟩
+  have hBJ : M.relRank B J = 0 := by
+    rw [<-indep_subset_maximal_iff_relrank_zero (hB.trans hA) hJ_subset hJ_indep]
+    unfold maximals; simp only [Set.mem_setOf_eq, and_imp]
+    exact ⟨⟨hJ_indep, hJ_subset⟩, hJ_max⟩
+  calc
+    M.relRank A B = M.relRank A B + M.relRank B J := by
+      rw [hBJ]; simp only [add_zero]
+    _ = M.relRank A J := by
+      exact eq_comm.mp (M.rel_rank_add_cancel hA hB hJ_subset)
+    _ = M.relRank A I + M.relRank I J := by
+      exact M.rel_rank_add_cancel hA hI_subset hJ
+    _ = M.relRank I J := by
+      rw [hAI]; simp only [zero_add]
 
 end RankMatroid
